interfaces: Do memory's API

examples/dynamic_isolation/Interfaces.v
@@ -588,8 +588,7 @@ Module Type Core_sig (External: External_sig) (Params: EnclaveParameters) (CoreP
           (reset_st: valid_reset_state st),
         valid_state st.
     *)
-
-  End CoreAxioms.
+  (* End CoreAxioms. *)
 
 End Core_sig.
 
@@ -1196,7 +1195,7 @@ Module Type Memory_sig (External: External_sig) (EnclaveParams: EnclaveParameter
 
   Declare Instance FiniteType_internal_reg_t : FiniteType internal_reg_t.
 
-  Inductive reg_t :=
+  Inductive external_reg_t :=
   | toIMem0 (state: MemReq.reg_t)
   | toIMem1 (state: MemReq.reg_t)
   | toDMem0 (state: MemReq.reg_t)
@@ -1207,10 +1206,9 @@ Module Type Memory_sig (External: External_sig) (EnclaveParams: EnclaveParameter
   | fromDMem1 (state: MemResp.reg_t)
   | purge0
   | purge1
-  | internal (r: internal_reg_t)
   .
 
-  Definition R (idx: reg_t) :=
+  Definition R_external (idx: external_reg_t) : type :=
     match idx with
     | toIMem0 st => MemReq.R st
     | toIMem1 st => MemReq.R st
@@ -1222,10 +1220,9 @@ Module Type Memory_sig (External: External_sig) (EnclaveParams: EnclaveParameter
     | fromDMem1 st => MemResp.R st
     | purge0 => enum_t purge_state
     | purge1 => enum_t purge_state
-    | internal st => R_internal st
     end.
 
-  Definition r (idx: reg_t) : R idx :=
+  Definition r_external (idx: external_reg_t) : R_external idx :=
     match idx with
     | toIMem0 st => MemReq.r st
     | toIMem1 st => MemReq.r st
@@ -1237,11 +1234,27 @@ Module Type Memory_sig (External: External_sig) (EnclaveParams: EnclaveParameter
     | fromDMem1 st => MemResp.r st
     | purge0 => value_of_bits (Bits.zero)
     | purge1 => value_of_bits (Bits.zero)
-    | internal st => r_internal st
     end.
 
+  Inductive reg_t :=
+  | external (r: external_reg_t)
+  | internal (r: internal_reg_t)
+  .
 
-  Declare Instance FiniteType_reg_t : FiniteType reg_t.
+  Definition R (idx: reg_t) : type :=
+    match idx with
+    | external r => R_external r
+    | internal r => R_internal r
+    end.
+
+  Definition r idx : R idx :=
+    match idx with
+    | external s => r_external s
+    | internal s => r_internal s
+    end.
+
+  Instance FiniteType_ext_reg_t : FiniteType external_reg_t := _.
+  Instance FiniteType_reg_t : FiniteType reg_t := _.
 
   Definition ext_fn_t := External.ext_fn_t.
   Definition Sigma := External.Sigma.
@@ -1253,15 +1266,61 @@ Module Type Memory_sig (External: External_sig) (EnclaveParams: EnclaveParameter
 
   Axiom schedule : Syntax.scheduler pos_t rule_name_t.
 
-  Section Semantics.
-    Definition koika_state_t : Type := env_t ContextEnv (fun idx: reg_t => R idx).
+  Import EnclaveInterface.
 
+  Scheme Equality for ind_core_id.
+
+  Section Taint.
+
+    Definition external_reg_to_taint (reg: external_reg_t) : ind_core_id:=
+      match reg with
+      | toIMem0 st => CoreId0
+      | toIMem1 st => CoreId1
+      | toDMem0 st => CoreId0
+      | toDMem1 st => CoreId1
+      | fromIMem0 st => CoreId0
+      | fromIMem1 st => CoreId1
+      | fromDMem0 st => CoreId0
+      | fromDMem1 st => CoreId1
+      | purge0 => CoreId0
+      | purge1 => CoreId1
+      end.
+
+  End Taint.
+
+  Section Interface.
+    Definition proj_log__ext (log: Log R ContextEnv) : Log R_external ContextEnv :=
+      ContextEnv.(create) (fun reg => ContextEnv.(getenv) log (external reg)).
+
+    Definition lift_ext_log (log: Log R_external ContextEnv) : Log R ContextEnv :=
+      ContextEnv.(create) (fun reg => match reg return (RLog (R reg)) with
+                                   | external s => ContextEnv.(getenv) log s
+                                   | _ => []
+                                   end).
+
+    Definition filter_ext_log (log: Log R_external ContextEnv) (core: ind_core_id) : Log R_external ContextEnv :=
+      ContextEnv.(create) (fun reg => if ind_core_id_beq (external_reg_to_taint reg) core
+                                   then ContextEnv.(getenv) log reg
+                                   else []).
+
+    Definition tau := Log R_external ContextEnv.
+    Definition trace := list tau.
+  End Interface.
+
+  Section CycleSemantics.
+    Definition koika_state_t : Type := env_t ContextEnv (fun idx: reg_t => R idx).
     Definition dram_t : Type := nat -> option data_t.
+
     Parameter internal_external_state_t : Type.
+    Parameter initial_internal_external_state : internal_external_state_t.
     Definition external_state_t : Type := dram_t * internal_external_state_t.
 
-    Definition state : Type := koika_state_t * external_state_t.
+    Definition initial_external_state (initial_dram: dram_t) : external_state_t :=
+      (initial_dram, initial_internal_external_state).
 
+    Definition state : Type := koika_state_t * external_state_t.
+    Definition initial_state (initial_dram: dram_t) : state :=
+      (ContextEnv.(create) r, initial_external_state initial_dram).
     Definition empty_log : Log R ContextEnv := log_empty.
 
     Definition koika_update_function : koika_state_t -> Log R ContextEnv -> Log R ContextEnv. Admitted.
@@ -1274,11 +1333,367 @@ Module Type Memory_sig (External: External_sig) (EnclaveParams: EnclaveParameter
       let koika_log := koika_update_function koika_st input_log in
       external_update_function (koika_st, ext_st) koika_log.
 
-    Definition do_step (st: state) (input_log: Log R ContextEnv) : state :=
-      let '(log, ext_st') := update_function st input_log in
-      (commit_update (fst st) log, ext_st').
-  End Semantics.
+    Record step_io :=
+      { step_input : Log R_external ContextEnv;
+        step_feedback : Log R_external ContextEnv
+      }.
 
+    Record ifc_io :=
+      { ifc_step : step_io;
+        ifc_input_config0 : option EnclaveInterface.enclave_config;
+        ifc_input_config1 : option EnclaveInterface.enclave_config;
+      }.
+
+    Definition get_input_config (step: ifc_io) (core: ind_core_id) : option EnclaveInterface.enclave_config :=
+      match core with
+      | CoreId0 => step.(ifc_input_config0)
+      | CoreId1 => step.(ifc_input_config1)
+      end.
+
+    Definition do_step__impl (st: state) (step: step_io) : state * Log R ContextEnv :=
+      let input := lift_ext_log step.(step_input) in
+      let '(output, ext_st') := update_function st input in
+      let final := log_app (lift_ext_log step.(step_feedback)) (log_app output input) in
+      ((commit_update (fst st) final, ext_st'), output).
+
+    Definition do_steps__impl (initial_dram: dram_t) (steps: list step_io)
+                             : state * list (Log R ContextEnv) :=
+      fold_left (fun '(st, evs) step =>
+                   let '(st', ev) := do_step__impl st step in
+                   (st', evs ++ [ev]))
+                steps (initial_state initial_dram, []).
+
+  End CycleSemantics.
+
+  Section TODO_MOVE.
+
+    Definition AND (Ps: list Prop) : Prop :=
+      List.fold_left and Ps True.
+
+    Definition bits_eqb {sz} (v1: bits_t sz) (v2: bits_t sz) : bool :=
+      N.eqb (Bits.to_N v1) (Bits.to_N v2).
+
+    Definition initial_enclave_config0 : enclave_config :=
+      {| eid := Enclave0;
+         shared_page  := false
+      |}.
+    Definition initial_enclave_config1 : enclave_config :=
+      {| eid := Enclave1;
+         shared_page  := false
+      |}.
+
+  End TODO_MOVE.
+
+  Section TODO_dram.
+    Definition enclave_base enc_id := Bits.to_nat (EnclaveParams.enclave_base enc_id).
+    Definition enclave_max enc_id := Bits.to_nat (Bits.plus (EnclaveParams.enclave_base enc_id)
+                                                            (EnclaveParams.enclave_size enc_id)).
+    Definition shared_base := Bits.to_nat EnclaveParams.shared_mem_base.
+    Definition shared_max := Bits.to_nat (Bits.plus EnclaveParams.shared_mem_base EnclaveParams.shared_mem_size).
+
+    Definition memory_map : Type := EnclaveInterface.mem_region -> dram_t.
+
+    Import EnclaveInterface.
+
+    Definition addr_in_region (region: mem_region) (addr: nat): bool :=
+      match region with
+      | MemRegion_Enclave eid =>
+          (enclave_base eid <=? addr) && (addr <? (enclave_max eid))
+      | MemRegion_Shared =>
+          (shared_base <=? addr) && (addr <? shared_max)
+      | MemRegion_Other => false
+      end.
+
+    Definition filter_dram : dram_t -> mem_region -> dram_t :=
+      fun dram region addr =>
+        if addr_in_region region addr then
+          dram addr
+        else None.
+
+    (* NOTE: the current representation of memory regions is probably non-ideal... *)
+    Definition get_dram : memory_map -> enclave_config -> dram_t :=
+      fun mem_map enclave_config addr =>
+        let enclave_region := MemRegion_Enclave enclave_config.(eid) in
+        if addr_in_region enclave_region addr then
+          (mem_map enclave_region) addr
+        else if enclave_config.(shared_page) && (addr_in_region MemRegion_Shared addr) then
+          (mem_map MemRegion_Shared) addr
+        else None.
+
+    Definition update_regions (config: enclave_config) (dram: dram_t)
+                              (regions: memory_map)
+                              : memory_map :=
+      fun region =>
+        if mem_region_beq region MemRegion_Shared && config.(shared_page) then
+          filter_dram dram MemRegion_Shared
+        else if mem_region_beq region (MemRegion_Enclave config.(eid)) then
+          filter_dram dram region
+        else regions region.
+
+  End TODO_dram.
+
+  Section Spec.
+
+    Record props_t :=
+      { P_input : Prop;
+        P_output : Prop;
+        P_feedback: Prop
+      }.
+    Definition valid_inputs (props: list props_t) :=
+      AND (List.map P_input props).
+    Definition valid_feedback (props: list props_t) :=
+      AND (List.map P_feedback props).
+    Definition valid_output (props: list props_t) :=
+      AND (List.map P_output props).
+
+    Definition trivial_props : props_t :=
+      {| P_input := True;
+         P_output := True;
+         P_feedback := True
+      |}.
+
+
+    (* Interface properties *)
+    Definition valid_input_log__common (input_log: Log R_external ContextEnv) : Prop.
+    Admitted.
+
+    Definition valid_output_log__common (output_log: Log R_external ContextEnv) : Prop.
+    Admitted.
+
+    Definition valid_feedback_log__common (log: Log R_external ContextEnv) : Prop :=
+      log = log_empty.
+
+    Import EnclaveInterface.
+
+    Inductive state_phase :=
+    | SpecSt_Running (config: enclave_config)
+    | SpecSt_Waiting.
+
+    Definition local_spec_state_t : Type := state * state_phase.
+
+    Record spec_state_t :=
+      { machine0 : local_spec_state_t;
+        machine1 : local_spec_state_t;
+        regions: memory_map;
+      }.
+
+    Definition initial_regions initial_dram : memory_map :=
+      fun region => filter_dram initial_dram region.
+
+    Definition initial_spec_state (initial_dram: dram_t) : spec_state_t :=
+      let mem0 := initial_state (initial_regions initial_dram (MemRegion_Enclave Enclave0)) in
+      let mem1 := initial_state (initial_regions initial_dram (MemRegion_Enclave Enclave1)) in
+      {| machine0 := (mem0, SpecSt_Running initial_enclave_config0);
+         machine1 := (mem1, SpecSt_Running initial_enclave_config1);
+         regions := initial_regions initial_dram
+      |}.
+
+    Definition external_state_is_reset (st: state) (core_id: ind_core_id): Prop :=
+      forall reg, external_reg_to_taint reg = core_id ->
+             ContextEnv.(getenv) (fst st) (external reg) = r_external reg.
+
+    Definition output_t := Log R_external ContextEnv.
+
+    Definition get_purge_reg (core: ind_core_id) : external_reg_t :=
+      match core with
+      | CoreId0 => purge0
+      | CoreId1 => purge1
+      end.
+
+    Definition get_dram_from_state (st: state) : dram_t :=
+      let '(_, (dram, _)) := st in dram.
+
+    (* TODO: infer this *)
+    Definition pf_R_ext_purge_reg: forall core,
+        (R (external (get_purge_reg core))) = enum_t purge_state.
+    Proof.
+      destruct core; reflexivity.
+    Defined.
+
+    Definition filter_step (step: step_io) (core: ind_core_id) : step_io :=
+      {| step_input := filter_ext_log (step_input step) core;
+         step_feedback := filter_ext_log (step_feedback step) core
+      |}.
+
+    Definition proj_ifc_io (step: ifc_io) (core: ind_core_id) : step_io * option enclave_config :=
+      (filter_step step.(ifc_step) core, get_input_config step core).
+
+    Definition do_local_step_trans__spec (machine: local_spec_state_t)
+                                       (core: ind_core_id)
+                                       (step: step_io)
+                                       (opt_config: option enclave_config)
+                                       (mem_map: memory_map)
+                                       : local_spec_state_t * output_t * memory_map :=
+      let '(st, phase) := machine in
+      let '(st', output) := do_step__impl st step in
+      let ext_output := proj_log__ext output in
+      let purge_reg := get_purge_reg core in
+      match phase with
+      | SpecSt_Running config =>
+          let continue := ((st', phase), ext_output, mem_map) in
+          let ext_st' := get_dram_from_state st' in
+          match rew_latest_write output (external purge_reg) (pf_R_ext_purge_reg core) with
+          | Some v => if bits_eqb v ENUM_purge_purged
+                     then ((st', SpecSt_Waiting), ext_output, update_regions config ext_st' mem_map)
+                     else continue
+          | None => continue
+          end
+      | SpecSt_Waiting =>
+          let continue := ((st', SpecSt_Waiting), ext_output, mem_map) in
+          let input_log := step.(step_input) in
+          match rew_latest_write input_log purge_reg (pf_R_ext_purge_reg core), opt_config with
+          | Some v, Some config =>
+             if bits_eqb v ENUM_purge_restart then
+               let dram := get_dram mem_map config in
+               ((initial_state dram, SpecSt_Running config), ext_output, mem_map)
+             else (* don't care *) continue
+          | _, _ => continue
+          end
+      end.
+
+    Definition do_step_trans__spec (spec_st: spec_state_t) (step: ifc_io)
+                                 : spec_state_t * output_t * output_t :=
+      let '(step0, config0) := proj_ifc_io step CoreId0 in
+      let '(step1, config1) := proj_ifc_io step CoreId1 in
+      let '(machine0', output0, mem_map') :=
+          do_local_step_trans__spec (machine0 spec_st) CoreId0 step0 config0 (regions spec_st) in
+      let '(machine1', output1, mem_map'') :=
+          do_local_step_trans__spec (machine1 spec_st) CoreId1 step1 config1 mem_map' in
+      ({| machine0 := machine0';
+          machine1 := machine1';
+          regions := mem_map'' |}, output0, output1).
+
+    Definition only_write_ext_purge (log: Log R_external ContextEnv) (core: ind_core_id) (v: bits_t 2) : Prop :=
+      let purge_reg := get_purge_reg core in
+         rew_latest_write log purge_reg (pf_R_ext_purge_reg core) = Some v
+      \/ latest_write log purge_reg = None.
+
+    (* addr req are in range *)
+    Definition mem_reqs_in_config (log: Log R_external ContextEnv) (config: enclave_config) (core: ind_core_id)
+                                  : Prop.
+    Admitted.
+
+    Definition disjoint_configs (opt_config0: option enclave_config) (opt_config1: option enclave_config) : Prop :=
+      match opt_config0, opt_config1 with
+      | Some config0, Some config1 =>
+          config0.(eid) <> config1.(eid) /\ (config0.(shared_page) && config1.(shared_page) = false)
+      | _, _ => True
+      end.
+
+    Definition valid_local_step_input (local_st: local_spec_state_t)
+                                      (core: ind_core_id)
+                                      (step: step_io)
+                                      (opt_config: option enclave_config)
+                                      (mem_map: memory_map)
+                                      : Prop :=
+      let '(st, phase) := local_st in
+      let '(st', output, _) := do_local_step_trans__spec local_st core step opt_config mem_map in
+      let purge := get_purge_reg core in
+      let input := step.(step_input) in
+      valid_input_log__common input /\
+      match phase with
+      | SpecSt_Running config =>
+          (* TODO: inputs belong to the enclave *)
+          only_write_ext_purge input core ENUM_purge_purging /\
+          opt_config = Some config /\
+          mem_reqs_in_config input config core
+      | SpecSt_Waiting =>
+          only_write_ext_purge input core ENUM_purge_restart /\
+          (rew_latest_write input purge (pf_R_ext_purge_reg core) = Some ENUM_purge_restart ->
+           opt_config <> None /\
+           external_state_is_reset (fst st') core (* TODO: whose responsibility to clear FIFOs? *)
+          )
+      end.
+
+    Definition valid_step_input__spec (spec_st: spec_state_t) (step: ifc_io) : Prop :=
+      let '(step0, config0) := proj_ifc_io step CoreId0 in
+      let '(step1, config1) := proj_ifc_io step CoreId1 in
+      let '(_, _, mem_map') :=
+          do_local_step_trans__spec (machine0 spec_st) CoreId0 step0 config0 (regions spec_st) in
+      valid_local_step_input (machine0 spec_st) CoreId0 step0 config0 (regions spec_st) /\
+      valid_local_step_input (machine1 spec_st) CoreId1 step1 config1 mem_map' /\
+      (* not same config *)
+      disjoint_configs config0 config1 /\
+      (* only one restart at a time *)
+      (not (latest_write step0.(step_input) purge0 = Some ENUM_purge_restart /\
+          latest_write step1.(step_input) purge1 = Some ENUM_purge_restart)) /\
+      valid_input_log__common step.(ifc_step).(step_input). (* TODO *)
+
+    (* Not very interesting: machine0 only outputs to external0; behaves like interface *)
+    Definition valid_step_output__spec (spec_st: spec_state_t) (step: ifc_io) : Prop.
+    Admitted.
+
+    Definition spec_output_t : Type := output_t * output_t.
+
+    Definition do_step__spec (spec_st: spec_state_t) (step: ifc_io)
+                           : spec_state_t * spec_output_t * props_t :=
+      let '(st', log0, log1) := do_step_trans__spec spec_st step in
+      let props' := {| P_input := valid_step_input__spec spec_st step;
+                       P_output := valid_step_output__spec spec_st step;
+                       P_feedback := valid_feedback_log__common step.(ifc_step).(step_feedback)
+                    |} in
+      (st', (log0, log1), props').
+
+    Definition do_steps__spec (initial_dram: dram_t) (steps: list ifc_io)
+                            : spec_state_t * list spec_output_t * list props_t :=
+      fold_left (fun '(st, evs0, props) step =>
+                   let '(st', ev0, prop) := do_step__spec st step in
+                   (st', evs0 ++ [ev0], props ++ [prop]))
+                steps (initial_spec_state initial_dram, [], []).
+
+  End Spec.
+
+  Section Correctness.
+
+    (* TODO: clean *)
+    Definition log_equivalent (koika_log: Log R ContextEnv) (spec_log: Log R_external ContextEnv) : Prop :=
+      forall (reg: external_reg_t),
+        latest_write koika_log (external reg) = latest_write spec_log reg /\
+        (forall port, may_read koika_log port (external reg) = may_read spec_log port reg) /\
+        (forall port, may_write koika_log log_empty port (external reg) =
+                 may_write spec_log log_empty port reg).
+
+    Definition tau_equivalent (impl_tau: Log R ContextEnv) (spec_tau: spec_output_t) : Prop :=
+      let (log0, log1) := spec_tau in
+      let spec_ext_log := ContextEnv.(create)
+                            (fun reg => match external_reg_to_taint reg with
+                                     | CoreId0 => ContextEnv.(getenv) log0 reg
+                                     | CoreId1 => ContextEnv.(getenv) log1 reg
+                                     end) in
+      log_equivalent impl_tau spec_ext_log.
+
+    Definition trace_equivalent (koika_tr: list (Log R ContextEnv))
+                                (spec_tr: list spec_output_t) : Prop :=
+      Forall2 tau_equivalent koika_tr spec_tr.
+
+    Axiom correctness :
+      forall (initial_dram: dram_t)
+        (steps: list ifc_io)
+        (spec_st: spec_state_t) (spec_tr: list spec_output_t) (props: list props_t)
+        (koika_st: state) (koika_tr: list (Log R ContextEnv)),
+      valid_inputs props ->
+      valid_feedback props ->
+      do_steps__spec initial_dram steps = (spec_st, spec_tr, props) ->
+      do_steps__impl initial_dram (List.map ifc_step steps) = (koika_st, koika_tr) ->
+      trace_equivalent koika_tr spec_tr.
+
+  End Correctness.
+
+  Section Compliance.
+    Axiom compliance:
+      forall (initial_dram: dram_t)
+        (steps: list ifc_io)
+        (spec_st: spec_state_t) (spec_tr: list spec_output_t) (props: list props_t)
+        (koika_st: state) (koika_tr: list (Log R ContextEnv)),
+      valid_inputs props ->
+      valid_feedback props ->
+      do_steps__spec initial_dram steps = (spec_st, spec_tr, props) ->
+      do_steps__impl initial_dram (List.map ifc_step steps) = (koika_st, koika_tr) ->
+      valid_output props.
+
+  End Compliance.
+
+  (*
   Section Taint.
     Inductive taint_t :=
     | TaintCore (id: ind_core_id)
@@ -1569,6 +1984,7 @@ k    Definition bits_eqb {sz} (v1: bits_t sz) (v2: bits_t sz) : bool :=
 
 
   End CycleModel.
+  *)
     (*
   Section Semantics.
     Definition state := env_t ContextEnv (fun idx : reg_t => R idx).
